state important hist lemmas

src/program_proof/pav/history.v
@@ -3,7 +3,7 @@ From Goose.github_com.mit_pdos.pav Require Import kt.
 
 From Perennial.program_proof.pav Require Import client core.
 
-Section core_iprop.
+Section defs.
 Context `{!heapGS Σ, !pavG Σ}.
 
 (* TODO: maybe only cliG version needed. not pure or adtrG. *)
@@ -30,36 +30,55 @@ Definition know_hist_val_cliG cli_γ (uid ep : w64) (lat : lat_val_ty) : iProp �
       "#Hsubmap" ∷ mono_list_idx_own cli_γ (uint.nat bound) (Some (dig, m_γ)) ∗
       "#Hin_bound" ∷ (uid, W64 $ length vals) ↪[m_γ] Some (bound, comm))).
 
-Definition know_hist_cliG cli_γ (uid : w64) (hist : list lat_val_ty) : iProp Σ :=
-  ([∗ list] ep ↦ lat ∈ hist, know_hist_val_cliG cli_γ uid (W64 ep) lat).
-
-End core_iprop.
-
-Section HistEntry.
-Context `{!heapGS Σ}.
-Definition own_HistEntry (ptr : loc) (obj : map_val_ty) : iProp Σ :=
-  ∃ sl_HistVal,
-  "Hptr_Epoch" ∷ ptr ↦[HistEntry :: "Epoch"] #obj.1 ∗
-  "Hptr_HistVal" ∷ ptr ↦[HistEntry :: "HistVal"] (slice_val sl_HistVal) ∗
-  "#Hsl_HistVal" ∷ own_slice_small sl_HistVal byteT DfracDiscarded obj.2.
-End HistEntry.
-
-Section hist.
-Context `{!heapGS Σ, !pavG Σ}.
-
 Definition get_lat (phys : list map_val_ty) (ep : w64) : lat_val_ty :=
   last $ filter (λ x, uint.Z x.1 ≤ uint.Z ep) phys.
 
 Definition phys_logic_reln phys (logic : list lat_val_ty) :=
   (∀ (ep : w64) lat, logic !! uint.nat ep = Some lat → lat = get_lat phys ep).
 
+(* know_hist_cliG ties together phys_hist and logic_hist as two different
+hist repr's, either of which may be convenient at any given time. *)
+Definition know_hist_cliG cli_γ (uid : w64) (phys_hist : list map_val_ty) (logic_hist : list lat_val_ty) : iProp Σ :=
+  ⌜ phys_logic_reln phys_hist logic_hist ⌝ ∗
+  ([∗ list] ep ↦ lat ∈ logic_hist, know_hist_val_cliG cli_γ uid (W64 ep) lat).
+
+Definition own_HistEntry (ptr : loc) (obj : map_val_ty) : iProp Σ :=
+  ∃ sl_HistVal,
+  "Hptr_Epoch" ∷ ptr ↦[HistEntry :: "Epoch"] #obj.1 ∗
+  "Hptr_HistVal" ∷ ptr ↦[HistEntry :: "HistVal"] (slice_val sl_HistVal) ∗
+  "#Hsl_HistVal" ∷ own_slice_small sl_HistVal byteT DfracDiscarded obj.2.
+
 Definition own_hist cli_γ uid sl_hist phys_hist : iProp Σ :=
   ∃ dim0_hist logic_hist,
   "Hsl_hist" ∷ own_slice sl_hist ptrT (DfracOwn 1) dim0_hist ∗
   "Hdim0_hist" ∷ ([∗ list] p;o ∈ dim0_hist;phys_hist, own_HistEntry p o) ∗
-  "%Hlogic_reln" ∷ ⌜ phys_logic_reln phys_hist logic_hist ⌝ ∗
-  "#Hknow_hist" ∷ know_hist_cliG cli_γ uid logic_hist.
-End hist.
+  "#Hknow_hist" ∷ know_hist_cliG cli_γ uid phys_hist logic_hist.
+
+Definition msv_final (adtr_γ : gname) (ep uid : w64) (lat : lat_val_ty) : iProp Σ.
+Admitted.
+End defs.
+
+Section derived.
+Context `{!heapGS Σ, !pavG Σ}.
+
+Lemma hist_extend_selfmon logic_hist ep cli_γ uid phys_hist :
+  (uint.Z $ length logic_hist) - 1 ≤ uint.nat ep →
+  ("#Hknow_hist" ∷ know_hist_cliG cli_γ uid phys_hist logic_hist ∗
+  "#His_bound" ∷ is_my_bound cli_γ uid (W64 $ length phys_hist) ep) -∗
+  ∃ new_hist,
+  "%Hlen_hist" ∷ ⌜ length new_hist = S $ uint.nat ep ⌝ ∗
+  "Hknow_hist" ∷ know_hist_cliG cli_γ uid phys_hist new_hist.
+Proof. Admitted.
+
+Lemma hist_audit_msv ep lat logic_hist aud_ep cli_γ uid phys_hist adtr_γ :
+  logic_hist !! uint.nat ep = Some lat →
+  length logic_hist ≤ aud_ep →
+  ("#Hknow_hist" ∷ know_hist_cliG cli_γ uid phys_hist logic_hist ∗
+  "#His_audit" ∷ is_audit cli_γ adtr_γ aud_ep) -∗
+  "#Hmsv" ∷ msv_final adtr_γ ep uid lat.
+Proof. Admitted.
+
+End derived.
 
 Section wps.
 Context `{!heapGS Σ, !pavG Σ}.
